feat: add caching for verified k-induction circuits (#1314)
This attempt uses a different strategy from the previous failed strategy
for caching. We show how to incrementally build our core circuits, and
maintain proofs that our circuits used for recursion are indeed the
outputs of calls to the core circuits, by using a `_succ` theorem that
tells us how to convert a circuit for steps upto `n` to a circuit for
upto steps `n+1`.

SSA/Experimental/Bits/Fast/ReflectVerif.lean
@@ -452,6 +452,17 @@ def castLe (i : Inputs ι n) (hn : n ≤ m) : Inputs ι m where
   ix := ⟨i.ix, by omega⟩
   input := i.input
 
+@[simp]
+theorem castLe_eq_self {α : Type _} {n : Nat} (i : Inputs α n) (h : n ≤ n) :
+    i.castLe h = i := by
+  simp [Inputs.castLe]
+
+@[simp]
+theorem castLe_castLe_eq_castLe {α : Type _} {p q r : Nat}
+  (i : Inputs α p) (h : p ≤ q) (h' : q ≤ r) :
+    (i.castLe h).castLe h' = i.castLe (by omega) := by
+  simp [Inputs.castLe]
+
 /-- casts bits in `[0..n)` to `[m-n..m)` by shifting the index. -/
 def castShift (i : Inputs ι n) (hn : n ≤ m) : Inputs ι m where
   ix := ⟨m - 1 - i.ix, by omega⟩
@@ -526,6 +537,24 @@ def Vars.castShift {n m : Nat} (v : Vars σ ι n) (hnm : n ≤ m) : Vars σ ι m
   match v with
   | .state s => .state s
   | .inputs is => .inputs (is.castShift hnm)
+
+/-- casting to the same width equals vars-/
+@[simp]
+theorem Vars.castLe_eq_self {α : Type _} {n : Nat} (v : Vars α σ n) (h : n ≤ n) :
+    v.castLe h = v := by
+  rcases v with x | i
+  · simp [Vars.castLe]
+  · simp [Vars.castLe]
+
+/-- casting to the same width equals vars-/
+@[simp]
+theorem Vars.castLe_castLe_eq_castLe_self {α : Type _} {p q r : Nat}
+  (v : Vars α σ p) (h : p ≤ q) (h' : q ≤ r) :
+    (v.castLe h).castLe h' = v.castLe (by omega) := by
+  rcases v with x | i
+  · simp [Vars.castLe]
+  · simp [Vars.castLe]
+
 
 /-- Relate boolean and bitstream environments. -/
 structure EnvOutRelated {arity : Type _} {α : Type _}
@@ -636,286 +665,6 @@ theorem EnvOutRelated_self_Bitstream_of_envBool
   intros x i hi
   simp [Bitstream_of_envBool, hi]
 
--- structure StateCircuit {arity : Type _}
---     [DecidableEq arity]
---     [Fintype arity]
---     [Hashable arity]
---     (p : FSM arity) (iter : Nat) where ofFun ::
---   toFun : p.α →  Circuit (Vars p.α arity iter)
-
--- /-- Product initial state vector,
--- that sets the state to be the intial state as given by the FSM.. -/
--- def StateCircuit.zero {arity : Type _}
---     [DecidableEq arity]
---     [Fintype arity]
---     [Hashable arity]
---     (p : FSM arity) : StateCircuit p 0 where
---   toFun :=
---     fun a => Circuit.ofBool (p.initCarry a)
-
--- @[simp]
--- theorem StateCircuit.zero_eval {arity : Type _}
---     [DecidableEq arity]
---     [Fintype arity]
---     [Hashable arity]
---     {p : FSM arity} {a : p.α} (envBool : Vars p.α arity 0 → Bool) :
---     ((StateCircuit.zero p).toFun a).eval envBool = p.initCarry a := by
---   simp only [zero, Circuit.ofBool]
---   rcases h : p.initCarry a <;> simp [h]
-
--- /-- Product free state vector, that reads state from the input.. -/
--- def StateCircuit.id  {arity : Type _}
---     [DecidableEq arity]
---     [Fintype arity]
---     [Hashable arity]
---     (p : FSM arity) : StateCircuit p 0 where
---   toFun :=
---     fun a => Circuit.var true (Vars.state a)
-
--- @[simp]
--- theorem StateCircuit.eval_id {arity : Type _}
---     [DecidableEq arity]
---     [Fintype arity]
---     [Hashable arity]
---     {p : FSM arity} {a : p.α} {envBool : Vars p.α arity 0 → Bool} :
---     ((StateCircuit.id p).toFun a).eval envBool = (envBool (Vars.state a)) := by
---   simp only [id, Circuit.ofBool]
---   rcases h : p.initCarry a <;> simp [h]
-
--- /-- Make a circuit for one step of transition.  -/
--- def StateCircuit.delta  {arity : Type _}
---     [DecidableEq arity]
---     [Fintype arity]
---     [Hashable arity]
---     (p : FSM arity) : StateCircuit p 1 where
---   toFun :=
---     fun a =>
---       let x := StateCircuit.id p
---       x.toFun a |>.bind fun v =>
---         match v with
---         | .state s =>
---           let d := p.nextBitCirc (some s)
---           d.map fun w =>
---             match w with
---             | .inl a => Vars.state a
---             | .inr i => Vars.inputs (Inputs.mk 0 i)
---         | .inputs i => i.elim0
-
--- @[simp]
--- theorem StateCircuit.eval_delta {arity : Type _}
---     [DecidableEq arity]
---     [Fintype arity]
---     [Hashable arity]
---     {p : FSM arity} {a : p.α} (envBool : Vars p.α arity 1 → Bool)
---     (envBitstream : arity → BitStream)
---     (hEnvBitstream : EnvOutRelated envBool envBitstream)
---     :
---     ((StateCircuit.delta p).toFun a).eval envBool =
---     p.delta (fun s => envBool (Vars.state s)) envBitstream a
---       := by
---   simp only [delta, Fin.isValue, Circuit.eval_bind, eval_id, FSM.delta_eq_carryWith_one]
---   simp only [Fin.isValue, FSM.carryWith]
---   simp only [Fin.isValue, Circuit.eval_map]
---   congr
---   ext x
---   rcases x with state | x
---   · simp only [FSM.carry_zero, FSM.initCarry_changeInitCarry_eq, Sum.elim_inl]
---   · simp only [Fin.isValue, FSM.carry_zero, FSM.initCarry_changeInitCarry_eq, Sum.elim_inr]
---     apply hEnvBitstream.envBool_inputs_mk_eq_envBitStream
-
--- /-- Allow state circuit to consume more inputs.  -/
--- def StateCircuit.castLe  {arity : Type _}
---     [DecidableEq arity]
---     [Fintype arity]
---     [Hashable arity]
---     {p : FSM arity}
---     (cn : StateCircuit p n)
---     (hnm : n ≤ m) :  StateCircuit p m where
---   toFun := fun state =>
---     (cn.toFun state).map fun v => v.castLe hnm
-
--- @[simp]
--- theorem StateCircuit.toFun_castLe {arity : Type _}
---     [DecidableEq arity]
---     [Fintype arity]
---     [Hashable arity]
---     {p : FSM arity} {n m : Nat} (cn : StateCircuit p n) (hnm : n ≤ m) :
---     (cn.castLe hnm).toFun = (fun i => (cn.toFun i).map (fun v => v.castLe hnm)) := rfl
-
--- /-- Move inputs from [0..n) to [d..d+n). -/
--- def StateCircuit.translateInputs {arity : Type _}
---     [DecidableEq arity]
---     [Fintype arity]
---     [Hashable arity]
---     {p : FSM arity}
---     (cn : StateCircuit p n)
---     (d : Nat) : StateCircuit p (d + n) where
---   toFun := fun state =>
---     (cn.toFun state).map fun v =>
---       match v with
---       | .state s => .state s
---       | .inputs i => .inputs (Inputs.mk ⟨i.ix + d, by omega⟩ i.input)
-
--- /-- Compose state circuits of 'n' steps and 'm' steps to get a circuit for 'n + m' steps. -/
--- def StateCircuit.compose {arity : Type _}
---     [DecidableEq arity]
---     [Fintype arity]
---     [Hashable arity]
---     {p : FSM arity}
---     /- Circuit that runs for [0..n) steps. -/
---     (sFst : StateCircuit p n)
---     /- Circuit that runs for [n..n+m ] steps. -/
---     (sSnd : StateCircuit p m) :
---     StateCircuit p (n + m) where
---   toFun := fun state =>
---     ((sSnd.translateInputs n).toFun state).bind fun v =>
---       match v with
---       | .state s =>
---           (sFst.castLe (show n ≤ n + m by omega)).toFun s
---       | .inputs i => Circuit.var .true (.inputs i)
-
--- /-- How to evaluate composition of circuits. -/
--- theorem StateCircuit.eval_compose {arity : Type _}
---     [DecidableEq arity]
---     [Fintype arity]
---     [Hashable arity]
---     {p : FSM arity} {a : p.α} (envBool : Vars p.α arity (n + m) → Bool)
---     (sFst : StateCircuit p n) (sSnd : StateCircuit p m)
---     :
---     ((StateCircuit.compose sFst sSnd).toFun a).eval envBool =
---       (sSnd.toFun a).eval (fun v =>
---         match v with
---         | .state s => (sFst.toFun s).eval (fun v => envBool (v.castLe (by omega)))
---         | .inputs i => envBool <| .inputs <| Inputs.mk ⟨i.ix + n, by omega⟩ i.input
---       ):= by
---   simp only [compose]
---   simp only [toFun_castLe, Circuit.eval_bind]
---   simp only [translateInputs]
---   simp only [Circuit.eval_map]
---   congr 1
---   ext i
---   rcases i with s | i
---   · simp only
---     simp only [Circuit.eval_map]
---   · simp only [Circuit.eval, ↓reduceIte]
-
--- /-- Build the output circuit from the given state circuit. -/
--- def StateCircuit.toOutput {arity : Type _}
---     [DecidableEq arity]
---     [Fintype arity]
---     [Hashable arity]
---     {p : FSM arity}
---     /- Circuit that runs for [0..n) steps. -/
---     (sc : StateCircuit p n)
---     /- Circuit that runs for [0..n+1] steps and produces an output. -/
---     : Circuit (Vars p.α arity (n + 1)) :=
---   (p.nextBitCirc none).bind fun v =>
---     match v with
---     | .inl s => (sc.castLe (by omega)).toFun s
---     | .inr i =>  Circuit.var true (Vars.inputs (Inputs.mk ⟨n, by omega⟩ i))
-
--- theorem StateCircuit.eval_toOutput_eq_
---     [DecidableEq arity]
---     [Fintype arity]
---     [Hashable arity]
---     {p : FSM arity} (envBool : Vars p.α arity (n + 1) → Bool)
---     -- (envBitstream : arity → BitStream)
---     -- (hEnvBitstream : EnvOutRelated envBool envBitstream)
---     (sc : StateCircuit p n)
---     :
---     (sc.toOutput).eval envBool =
---     ((p.nextBitCirc none).eval (fun x =>
---       match x with
---       | .inl s => (sc.toFun s).eval (fun i => envBool <| i.castLe (by omega))
---       | .inr i => envBool <| Vars.inputs (Inputs.mk ⟨n, by omega⟩ i))) := by
---   simp only [toOutput, toFun_castLe]
---   simp only [Circuit.eval_bind]
---   congr
---   ext x
---   rcases x with s | i
---   · simp  [Circuit.eval_map]
---   · simp
-
--- @[simp]
--- theorem StateCircuit.eval_toOutput_eq
---     [DecidableEq arity]
---     [Fintype arity]
---     [Hashable arity]
---     {p : FSM arity} (envBool : Vars p.α arity (n + 1) → Bool)
---     (sc : StateCircuit p n)
---     :
---     (sc.toOutput).eval envBool =
---     p.outputWith
---       (fun s => (sc.toFun s).eval (fun i => envBool <| i.castLe (by omega)))
---       (fun i => envBool <| Vars.inputs (Inputs.mk ⟨n, by omega⟩ i)) := by
---   simp only [toOutput, toFun_castLe]
---   simp only [Circuit.eval_bind]
---   congr
---   ext x
---   rcases x with s | i
---   · simp  [Circuit.eval_map]
---   · simp
-
-
--- /-- Build the circuit for n transitions.-/
--- def StateCircuit.deltaN  {arity : Type _}
---     [DecidableEq arity]
---     [Fintype arity]
---     [Hashable arity]
---     (p : FSM arity)
---     (n : Nat) : StateCircuit p n :=
---   match n with
---   | 0 => StateCircuit.id p
---   | n' + 1 =>
---     let d := (StateCircuit.delta p)
---     let sn := StateCircuit.deltaN p n'
---     (d.compose sn).castLe (by omega)
-
--- @[simp]
--- theorem StateCircuit.eval_deltaN_eq {arity : Type _}
---   [DecidableEq arity]
---   [Fintype arity]
---   [Hashable arity]
---   {p : FSM arity} (envBool : Vars p.α arity n → Bool)
---   (envBitstream : arity → BitStream)
---   (hEnvBitstream : EnvOutRelated envBool envBitstream)
---   (s : p.α)
---   :
---   ((StateCircuit.deltaN p n).toFun s).eval envBool =
---     p.carryWith (fun s => envBool <| .state s) envBitstream n s := by
---   induction n
---   case zero =>
---     simp [StateCircuit.deltaN, StateCircuit.id, Circuit.eval_map]
---   sorry
-
-
--- /-- Make circuit that produces output for index 'i'. -/
--- def StateCircuit.deltaNOutput {arity : Type _}
---   [DecidableEq arity]
---   [Fintype arity]
---   [Hashable arity]
---   (p : FSM arity) (n : Nat) (i : Nat)  (hin : i ≤ n): (Circuit (Vars p.α arity (n+1))) :=
---   ((StateCircuit.deltaN p i).castLe (show i ≤ n by omega)).toOutput
-
--- @[simp]
--- theorem StateCircuit.eval_deltaNOutput_eq
---     {arity : Type _}
---     [DecidableEq arity]
---     [Fintype arity]
---     [Hashable arity]
---     (p : FSM arity) (n : Nat) (i : Nat) (hin : i ≤ n)
---     (envBool : Vars p.α arity (n + 1) → Bool)
---     (envBitstream : arity → BitStream)
---     (envInit : p.α → Bool)
---     (hEnvInit : envInit = initCarry_of_envBool envBool)
---     (hEnvBitstream : EnvOutRelated envBool envBitstream)
---     :
---     (deltaNOutput p n i hin).eval envBool = p.evalWith envInit envBitstream i := by
---   rw [deltaNOutput]
---   simp only [eval_toOutput_eq, toFun_castLe]
---   sorry
-
-
 /-- Take the 'or' of many circuits.-/
 def Circuit.bigOr {α : Type _}
     (cs : List (Circuit α)) : Circuit α :=
@@ -923,6 +672,57 @@ def Circuit.bigOr {α : Type _}
   | [] => Circuit.fals
   | c :: cs =>
     c ||| (Circuit.bigOr cs)
+
+@[simp]
+theorem Circuit.bigOr_nil_eq {α : Type _} :
+    Circuit.bigOr (α := α) [] = Circuit.fals := by
+  simp [bigOr]
+
+@[simp]
+theorem Circuit.bigOr_cons_eq {α : Type _}
+    (c : Circuit α) (cs : List (Circuit α)) :
+    Circuit.bigOr (c :: cs) = c ||| Circuit.bigOr cs := by
+  induction cs
+  case nil => simp [bigOr]
+  case cons a as ih =>
+    simp [bigOr, ih]
+
+
+/-- append to the bigOr list is equivalent to a circuit
+that is the bigOr of the circuit and the |||
+-/
+theorem Circuit.bigOr_append_equiv_or_bigOr {α : Type _}
+    (c : Circuit α) (cs : List (Circuit α)) :
+    Circuit.Equiv (Circuit.bigOr (cs ++ [c])) (c ||| Circuit.bigOr cs) := by
+  induction cs
+  case nil => simp [bigOr]
+  case cons a as ih =>
+    simp [bigOr, ih]
+    ext env
+    have := Circuit.eval_eq_of_Equiv ih
+    simp
+    rw [this]
+    simp [Circuit.eval_or]
+    rcases (a.eval env) <;> simp
+-- bigOr [a, b]
+-- = a ||| (bigOr [b])
+-- = a ||| (b ||| fals)
+
+theorem Circuit.bigOr_append_equiv_bigOr_cons {α : Type _}
+    (c : Circuit α) (cs : List (Circuit α)) :
+    Circuit.Equiv (Circuit.bigOr (cs ++ [c])) (Circuit.bigOr (c :: cs)) := by
+  rw [Circuit.bigOr_cons_eq]
+  apply Circuit.Equiv_trans
+  · apply Circuit.bigOr_append_equiv_or_bigOr
+  · apply Circuit.Equiv_refl
+
+theorem Circuit.eval_bigOr_eq_decide
+    (cs : List (Circuit α)) (env : α → Bool):
+    (Circuit.bigOr cs).eval env = decide (∃ c ∈ cs, c.eval env = true) := by
+  induction cs
+  case nil => simp [bigOr]
+  case cons a as ih =>
+    simp [bigOr, ih]
 
 @[simp]
 theorem Circuit.eval_bigOr_eq_false_iff
@@ -943,6 +743,73 @@ theorem Circuit.eval_bigOr_eq_true_iff
   case nil => simp [bigOr]
   case cons a as ih =>
     simp [bigOr, ih]
+
+def Circuit.bigOr' {α : Type _}
+    (cs : List (Circuit α)) : Circuit α :=
+  go cs Circuit.fals where
+  go : List (Circuit α) → Circuit α → Circuit α
+  | [], acc => acc
+  | c :: cs, acc =>
+    go cs (c ||| acc)
+-- go [a, b] fals
+-- = go [b] (a ||| fals)
+-- = go [] (b ||| (a ||| fals))
+-- = b ||| (a ||| fals)
+
+
+@[simp]
+theorem Circuit.bigOr'.go_append_eq {α : Type _}
+    (c : Circuit α) (cs : List (Circuit α)) (acc : Circuit α):
+    Circuit.bigOr'.go (cs ++ [c]) acc = c ||| Circuit.bigOr'.go cs acc := by
+  induction cs generalizing acc
+  case nil => simp [bigOr', bigOr'.go]
+  case cons a as ih =>
+    simp [bigOr', bigOr'.go, ih]
+
+theorem Circuit.bigOr'.append_eq {α : Type _}
+    (c : Circuit α) (cs : List (Circuit α)):
+    Circuit.bigOr' (cs ++ [c]) = c ||| Circuit.bigOr' cs := by
+  simp [bigOr', bigOr'.go_append_eq]
+
+theorem Circuit.bigOr'.go_eval_eq_false_iff
+    (cs : List (Circuit α)) (acc : Circuit α) (env : α → Bool):
+    (Circuit.bigOr'.go cs acc).eval env = false ↔
+    ((∀ (c : Circuit α), c ∈ cs → c.eval env = false) ∧ acc.eval env = false) := by
+  induction cs generalizing acc
+  case nil => simp [bigOr'.go]
+  case cons a as ih =>
+    simp [bigOr', bigOr'.go, go, ih]
+    tauto
+
+theorem Circuit.bigOr'.go_eval_eq_true_iff
+    (cs : List (Circuit α)) (acc : Circuit α) (env : α → Bool):
+    (Circuit.bigOr'.go cs acc).eval env = true ↔
+    ((∃ (c : Circuit α), c ∈ cs ∧ c.eval env = true) ∨ acc.eval env = true) := by
+  induction cs generalizing acc
+  case nil => simp [bigOr'.go]
+  case cons a as ih =>
+    simp [bigOr', bigOr'.go, go, ih]
+    constructor
+    · intros h
+      rcases h with h | h | h <;> simp [h]
+    · intros h
+      rcases h with (h | h) | h <;> simp [h]
+
+theorem Circuit.eval_bigOr'eq_false_iff
+    (cs : List (Circuit α)) (env : α → Bool):
+    (Circuit.bigOr' cs).eval env = false ↔
+    (∀ (c : Circuit α), c ∈ cs → c.eval env = false) := by
+  rw [bigOr']
+  rw [Circuit.bigOr'.go_eval_eq_false_iff]
+  simp
+
+theorem Circuit.bigOr'_eval_eq_true_iff
+    (cs : List (Circuit α)) (env : α → Bool):
+    (Circuit.bigOr' cs).eval env = true ↔
+    (∃ (c : Circuit α), c ∈ cs ∧ c.eval env = true) := by
+  rw [bigOr']
+  rw [Circuit.bigOr'.go_eval_eq_true_iff]
+  simp [Circuit.eval]
 
 /-- Take the and of many circuits.-/
 def Circuit.bigAnd {α : Type _}
@@ -978,7 +845,7 @@ theorem Circuit.eval_bigAnd_eq_false_iff
 Make the circuit that produces the state vector after 'n' iterations.
 This needs 'n' bits of input.
 -/
-def mkRealStateVectorCircuit {arity : Type _}
+def mkCarryCircuit {arity : Type _}
   [DecidableEq arity]
   [Fintype arity]
   [Hashable arity]
@@ -988,13 +855,13 @@ def mkRealStateVectorCircuit {arity : Type _}
   | n + 1 =>
     (p.nextBitCirc (some s)).bind fun v =>
       match v with
-      | .inl s' => (mkRealStateVectorCircuit p n s').map fun w =>
+      | .inl s' => (mkCarryCircuit p n s').map fun w =>
         match w with
         | .state s'' => Vars.state s''
         | .inputs i => Vars.inputs (Inputs.mk (i.ix) i.input)
       | .inr a => Circuit.var true (Vars.inputs (Inputs.mk ⟨n, by omega⟩ a))
 
-theorem mkRealStateVectorCircuit_eval_eq {arity : Type _}
+theorem mkCarryCircuit_eval_eq {arity : Type _}
     [DecidableEq arity]
     [Fintype arity]
     [Hashable arity]
@@ -1002,14 +869,14 @@ theorem mkRealStateVectorCircuit_eval_eq {arity : Type _}
     (envBool : Vars Empty arity n → Bool)
     (envBitstream : arity → BitStream)
     (hEnvBitstream : EnvOutRelated envBool envBitstream) :
-  (mkRealStateVectorCircuit p n s).eval envBool =
+  (mkCarryCircuit p n s).eval envBool =
   p.carryWith (fun s => p.initCarry s) envBitstream n s := by
   induction n generalizing s
   case zero =>
-    simp only [mkRealStateVectorCircuit, Circuit.ofBool, FSM.carryWith_zero_eq]
+    simp only [mkCarryCircuit, Circuit.ofBool, FSM.carryWith_zero_eq]
     rcases h : p.initCarry s <;> simp [h]
   case succ m hm =>
-    simp only [mkRealStateVectorCircuit, Fin.coe_eq_castSucc, Circuit.eval_bind,
+    simp only [mkCarryCircuit, Fin.coe_eq_castSucc, Circuit.eval_bind,
       FSM.carryWith_initCarry_eq_carry]
     simp only [FSM.carry, FSM.nextBit]
     congr
@@ -1029,214 +896,70 @@ theorem mkRealStateVectorCircuit_eval_eq {arity : Type _}
 
 
 /--
-Make the circuit that produces the output value after 'n' iterations.
-This needs 'n+1' bits of input.
--/
-def mkEvalCircuit {arity : Type _}
-    [DecidableEq arity]
-    [Fintype arity]
-    [Hashable arity]
-    (p : FSM arity) (n : Nat) : Circuit (Vars Empty arity (n+1)) :=
-  p.nextBitCirc none |>.bind fun v =>
-    match v with
-    | .inl s => (mkRealStateVectorCircuit p n s).map fun w =>
-      match w with
-      | .state s' => Vars.state s'
-      | .inputs i => Vars.inputs (Inputs.mk ⟨i.ix, by omega⟩ i.input)
-    | .inr a => Circuit.var true (Vars.inputs (Inputs.mk ⟨n, by omega⟩ a))
-
-@[simp]
-theorem eval_mkEvalCircuit_eq_false_iff
-    {arity : Type _}
-    [DecidableEq arity]
-    [Fintype arity]
-    [Hashable arity]
-    (p : FSM arity) (n : Nat)
-    (envBool : Vars Empty arity (n + 1) → Bool)
-    (envBitstream : arity → BitStream)
-    (hEnvBitstream : EnvOutRelated envBool envBitstream) :
-    -- Make a safety circuit, that computes the evaluation of the FSM.
-    (mkEvalCircuit p n).eval envBool =
-      p.eval envBitstream n  := by
-  simp [mkEvalCircuit]
-  simp [Circuit.eval_bind]
-  rw [FSM.eval, FSM.nextBit]
-  simp
-  congr
-  ext x
-  rcases x with a | i
-  · simp [Circuit.eval_map]
-    rw [mkRealStateVectorCircuit_eval_eq (envBitstream := envBitstream)]
-    · simp
-    · -- TODO: write this as a theorem that encapsulates that environments are related
-      -- upon casting of the input.
-      constructor
-      intros x i hi
-      simp only [Fin.castSucc_mk]
-      apply hEnvBitstream.envBool_inputs_mk_eq_envBitStream
-  · simp [initCarry_of_envBool]
-    apply hEnvBitstream.envBool_inputs_mk_eq_envBitStream
-
-/--
-info: 'ReflectVerif.BvDecide.eval_mkEvalCircuit_eq_false_iff' depends on axioms: [propext, Quot.sound]
--/
-#guard_msgs in #print axioms eval_mkEvalCircuit_eq_false_iff
-
-
--- /-
--- Make the safety circuit at index 'i',
--- which runs the program at the initial state on the inputs.
--- See that this fixes the state to 'Empty'.
--- -/
--- def mkSafetyCircuitAuxElem {arity : Type _}
---   [DecidableEq arity]
---   [Fintype arity]
---   [Hashable arity]
---   (p : FSM arity) (n : Nat) (i : Nat) (hin : i ≤ n) : (Circuit (Vars Empty arity (n+1))) :=
---   (StateCircuit.deltaNOutput p n i (by omega)).bind fun v =>
---     match v with
---     | .state s => Circuit.ofBool <| p.initCarry s
---     | .inputs i => Circuit.var true (.inputs i)
-
-
--- @[simp]
--- theorem eval_mkSafetyCircuitAuxElem_eq_false_iff
---     {arity : Type _}
---     [DecidableEq arity]
---     [Fintype arity]
---     [Hashable arity]
---     (p : FSM arity) (n : Nat) (i : Nat) (hin : i ≤ n)
---     (envBool : Vars Empty arity (n + 1) → Bool)
---     (envBitstream : arity → BitStream)
---     (hEnvBitstream : EnvOutRelated envBool envBitstream) :
---     (mkEvalCircuit p n).eval envBool =
---     p.eval envBitstream n = false := by
-
-/-- Make the list of safety circuits upto length 'n + 1'. -/
-def mkSafetyCircuitAuxList {arity : Type _}
-    [DecidableEq arity]
-    [Fintype arity]
-    [Hashable arity]
-    (p : FSM arity) (n : Nat) :
-    List (Circuit (Vars Empty arity (n+1))) :=
-  let ys := (List.range (n+1)).attach
-  ys.map fun i =>
-    (mkEvalCircuit p i.val).map (fun vs => vs.castLe (by
-      have := i.property; simp at this; omega
-    ))
-
-/--
-make the circuit that witnesses safety for (n+1) steps.
-This builds the safety circuit for 'n+1' steps, and takes the 'or' of all of these.
--/
-def mkSafetyCircuit {arity : Type _}
-  [DecidableEq arity] [Fintype arity] [Hashable arity]
-  (p : FSM arity) (n : Nat) : Circuit (Vars Empty arity (n+1)) :=
-  Circuit.bigOr (mkSafetyCircuitAuxList p n)
-
-/--
-Evaluating the safety circuit is false iff
-the bitstreams are false upto index 'n'.
--/
-theorem eval_mkSafetyCircuit_eq_false_iff_ {arity : Type _}
-    [DecidableEq arity] [Fintype arity] [Hashable arity]
-    (p : FSM arity) (n : Nat)
-    (envBool : Vars Empty arity (n + 1) → Bool)
-    (envBitstream : arity → BitStream)
-    (hEnvBitstream : EnvOutRelated envBool envBitstream) :
-    (mkSafetyCircuit p n).eval envBool = false ↔
-    (∀ (i : Nat), i ≤ n → p.eval envBitstream i = false) := by
-  rw [mkSafetyCircuit]
-  rw [Circuit.eval_bigOr_eq_false_iff]
-  rw [mkSafetyCircuitAuxList]
-  simp
-  constructor
-  · intros hc i hi
-    specialize hc _ i (by omega) rfl
-    simp [Circuit.eval_map] at hc
-    rw [eval_mkEvalCircuit_eq_false_iff
-      (envBitstream := envBitstream)
-    ] at hc
-    · apply hc
-    · -- TODO: write this as a theorem that encapsulates that environments are related
-      -- upon casting of the input.
-      constructor
-      intros x j hj
-      apply hEnvBitstream.envBool_inputs_mk_eq_envBitStream
-  · intros heval circ i hi hCirc
-    subst hCirc
-    simp [Circuit.eval_map]
-    rw [eval_mkEvalCircuit_eq_false_iff]
-    · apply heval
-      omega
-    · constructor
-      intros x j hj
-      apply hEnvBitstream.envBool_inputs_mk_eq_envBitStream
-
-/--
-info: 'ReflectVerif.BvDecide.eval_mkSafetyCircuit_eq_false_iff_' depends on axioms: [propext, Quot.sound]
--/
-#guard_msgs in #print axioms eval_mkSafetyCircuit_eq_false_iff_
-
-/--
-Evaluating the safety circuit is false iff
-the bitstreams are false upto index 'n'.
--/
-theorem eval_mkSafetyCircuit_eq_false_iff {arity : Type _}
-    [DecidableEq arity] [Fintype arity] [Hashable arity]
-    (p : FSM arity) (n : Nat) :
-    (∀ envBool, (mkSafetyCircuit p n).eval envBool = false) ↔
-    (∀ envBitstream, ∀ (i : Nat), i ≤ n → p.eval envBitstream i = false) := by
-  constructor
-  · intros h envBitstream i  hi
-    let envBool := envBoolEmpty_of_envBitstream envBitstream n
-    specialize h envBool
-    rw [eval_mkSafetyCircuit_eq_false_iff_
-      (envBitstream := envBitstream)
-    ] at h
-    · apply h
-      omega
-    · simp [envBool]
-  · intros h envBool
-    rw [eval_mkSafetyCircuit_eq_false_iff_
-      (envBitstream := Bitstream_of_envBool envBool)
-    ]
-    · intros i hi
-      apply h (Bitstream_of_envBool envBool) i hi
-    · simp
-
-/--
-info: 'ReflectVerif.BvDecide.eval_mkSafetyCircuit_eq_false_iff' depends on axioms: [propext, Quot.sound]
--/
-#guard_msgs in #print axioms eval_mkSafetyCircuit_eq_false_iff
-
-/-! ## Arbitrary State Vector Builder
-
-This section builds a circuit that produces the state vector after 'n' iterations,
-starting with a state vector that is given by the circuit itself.
-
--/
-/--
 Make the circuit that produces the state vector after 'n' iterations,
 starting with a state vector that is given by the circuit itself.
 -/
-def mkStateVectorWithCircuit {arity : Type _}
+def mkCarryWithCircuit {arity : Type _}
   [DecidableEq arity]
   [Fintype arity]
   [Hashable arity]
   (p : FSM arity) (n : Nat) : p.α → Circuit (Vars p.α arity n) := fun s =>
   match n with
   | 0 => Circuit.var true (Vars.state s)
-  | n + 1 =>
+  | k + 1 =>
     (p.nextBitCirc (some s)).bind fun v =>
       match v with
-      | .inl s' => (mkStateVectorWithCircuit p n s').map fun w =>
+      | .inl s' => (mkCarryWithCircuit p k s').map fun w =>
+        match w with
+        | .state s'' => Vars.state s''
+        | .inputs i => Vars.inputs (Inputs.mk (i.ix) i.input)
+      | .inr a => Circuit.var true (Vars.inputs (Inputs.mk ⟨k, by omega⟩ a))
+
+/-- make the CarryWith circuit at step 0. -/
+def mkCarryWith0Circuit {arity : Type _}
+    [DecidableEq arity]
+    [Fintype arity]
+    [Hashable arity]
+    (p : FSM arity) :
+    { f : p.α → Circuit (Vars p.α arity 0) //
+      ∀ (a : p.α), Circuit.Equiv (f a) (mkCarryWithCircuit p 0 a) } :=
+  ⟨mkCarryWithCircuit p 0, by simp⟩
+
+/--
+make the CarryWith circuit for step (n+1), incrementally,
+using the carryWith circuit at step n.
+-/
+def mkCarryWithSuccCircuit {arity : Type _}
+    [DecidableEq arity]
+    [Fintype arity]
+    [Hashable arity]
+    (p : FSM arity) (n : Nat)
+    (carryN : p.α → Circuit (Vars p.α arity n))
+    (hCarryN : ∀ (a : p.α), Circuit.Equiv (carryN a) (mkCarryWithCircuit p n a)) :
+    { f : p.α → Circuit (Vars p.α arity (n + 1)) //
+      ∀ (a : p.α), Circuit.Equiv (f a) (mkCarryWithCircuit p (n + 1) a) } where
+  val := fun s =>
+    (p.nextBitCirc (some s)).bind fun v =>
+      match v with
+      | .inl s' => (carryN s').map fun w =>
         match w with
         | .state s'' => Vars.state s''
         | .inputs i => Vars.inputs (Inputs.mk (i.ix) i.input)
       | .inr a => Circuit.var true (Vars.inputs (Inputs.mk ⟨n, by omega⟩ a))
+  property := by
+    intros a
+    ext env
+    rw [mkCarryWithCircuit]
+    simp
+    simp [Circuit.eval_bind]
+    congr 1
+    ext v
+    rcases v with a' | i
+    · simp [Circuit.eval_map]
+      rw [hCarryN]
+    · simp
 
-theorem eval_mkStateVectorWithCircuit_eq_carryWith {arity : Type _}
+theorem eval_mkCarryWithCircuit_eq_carryWith {arity : Type _}
     [DecidableEq arity]
     [Fintype arity]
     [Hashable arity]
@@ -1244,14 +967,14 @@ theorem eval_mkStateVectorWithCircuit_eq_carryWith {arity : Type _}
     (envBool : Vars p.α arity n → Bool)
     (envBitstream : arity → BitStream)
     (hEnvBitstream : EnvOutRelated envBool envBitstream) :
-  (mkStateVectorWithCircuit p n s).eval envBool =
+  (mkCarryWithCircuit p n s).eval envBool =
   p.carryWith (fun s => envBool (Vars.state s)) envBitstream n s := by
   induction n generalizing s
   case zero =>
-    simp only [mkStateVectorWithCircuit, Circuit.ofBool, FSM.carryWith_zero_eq]
+    simp only [mkCarryWithCircuit, Circuit.ofBool, FSM.carryWith_zero_eq]
     rcases h : envBool (Vars.state s) <;> simp [h]
   case succ m hm =>
-    simp only [mkStateVectorWithCircuit, Fin.coe_eq_castSucc, Circuit.eval_bind,
+    simp only [mkCarryWithCircuit, Fin.coe_eq_castSucc, Circuit.eval_bind,
       FSM.carryWith_initCarry_eq_carry]
     congr
     ext x
@@ -1268,6 +991,7 @@ theorem eval_mkStateVectorWithCircuit_eq_carryWith {arity : Type _}
     · simp only [Circuit.eval, ↓reduceIte, Sum.elim_inr]
       apply hEnvBitstream.envBool_inputs_mk_eq_envBitStream
 
+
 /-
 Make the safety circuit at index 'i',
 which runs the program at the initial state on the inputs.
@@ -1280,11 +1004,39 @@ def mkEvalWithCircuit {arity : Type _}
   (p : FSM arity) (n : Nat) : (Circuit (Vars p.α arity (n+1))) :=
   p.nextBitCirc none |>.bind fun v =>
     match v with
-    | .inl s => (mkStateVectorWithCircuit p n s).map fun w =>
+    | .inl s => (mkCarryWithCircuit p n s).map fun w =>
       match w with
       | .state s' => Vars.state s'
       | .inputs i => Vars.inputs (Inputs.mk ⟨i.ix, by omega⟩ i.input)
     | .inr a => Circuit.var true (Vars.inputs (Inputs.mk ⟨n, by omega⟩ a))
+
+/-- Make the circuit that evaluates to the initial state. -/
+def mkEvalWithCircuit_of_mkCarryWithCircuit {arity : Type _}
+    [DecidableEq arity]
+    [Fintype arity]
+    [Hashable arity]
+    (p : FSM arity) (n : Nat)
+    (carryN : p.α → Circuit (Vars p.α arity n))
+    (hCarryN : ∀ (a : p.α), Circuit.Equiv (carryN a) (mkCarryWithCircuit p n a)) :
+    { c : Circuit (Vars p.α arity (n + 1)) //
+      Circuit.Equiv c (mkEvalWithCircuit p n) } where
+  val :=   p.nextBitCirc none |>.bind fun v =>
+    match v with
+    | .inl s => (carryN s).map fun w =>
+      match w with
+      | .state s' => Vars.state s'
+      | .inputs i => Vars.inputs (Inputs.mk ⟨i.ix, by omega⟩ i.input)
+    | .inr a => Circuit.var true (Vars.inputs (Inputs.mk ⟨n, by omega⟩ a))
+  property := by
+    ext v
+    rw [mkEvalWithCircuit]
+    simp [Circuit.eval_bind]
+    congr
+    ext x
+    rcases x with a | i
+    · simp [Circuit.eval_map]
+      rw [hCarryN]
+    · simp
 
 @[simp]
 theorem eval_mkEvalWithCircuit_eq
@@ -1306,7 +1058,7 @@ theorem eval_mkEvalWithCircuit_eq
   ext x
   rcases x with a | i
   · simp [Circuit.eval_map, Sum.elim_inl]
-    rw [eval_mkStateVectorWithCircuit_eq_carryWith]
+    rw [eval_mkCarryWithCircuit_eq_carryWith]
     · rw [FSM.carryWith]
     · -- TODO extract out into generic theory.
       constructor
@@ -1331,6 +1083,76 @@ def mkEvalWithNCircuit {arity : Type _}
   [DecidableEq arity] [Fintype arity] [Hashable arity]
   (p : FSM arity) (n : Nat) : Circuit (Vars p.α arity (n+1)) :=
   Circuit.bigOr (mkEvalWithNCircuitAuxList p n)
+
+/-- mkEvalWithNCircuit evaluated at (n + 1) equals
+mkEvalWithNCircuit evaluated at n, or'd with
+mkEvalWithCircuit evaluated at (n + 1). -/
+theorem mkEvalWithNCircuit_succ_Eqiv_mkEvalWithNCircuit_or {arity : Type _}
+    [DecidableEq arity] [Fintype arity] [Hashable arity]
+    (p : FSM arity) (n : Nat) :
+    Circuit.Equiv
+      (mkEvalWithNCircuit p (n + 1))
+      ((mkEvalWithNCircuit p n).map (fun v => v.castLe (by omega)) ||| (mkEvalWithCircuit p (n + 1))) := by
+  simp [mkEvalWithNCircuit, mkEvalWithNCircuitAuxList]
+  ext env
+  rw [NNF.bool_eq_iff]
+  rw [Circuit.eval_bigOr_eq_true_iff]
+  simp [Circuit.eval_map]
+  constructor
+  · intros h
+    obtain ⟨hc, a, ha⟩ := h
+    obtain ⟨i, hi⟩ := a
+    obtain ⟨j, hj⟩ := hi
+    subst hj
+    simp [Circuit.eval_map] at ha
+    by_cases hi : i = n + 1
+    · subst hi
+      right
+      rw [← ha]
+      simp
+    · left
+      exists (mkEvalWithCircuit p i).map (fun v => v.castLe (by omega))
+      constructor
+      · exists i
+        exists (by omega)
+      · simp [Circuit.eval_map, ha]
+  · intros h
+    rcases h with h | h
+    · obtain ⟨c, ⟨⟨i, hi, hc'⟩, hc⟩ ⟩ := h
+      subst hc'
+      simp [Circuit.eval_map] at hc ⊢
+      exists (mkEvalWithCircuit p i).map (fun v => v.castLe (by omega))
+      constructor
+      · exists i
+        exists (by omega)
+      · simp [Circuit.eval_map, hc]
+    · exists (mkEvalWithCircuit p (n + 1)).map (fun v => v.castLe (by omega))
+      simp [h]
+      exists (n + 1)
+      exists (by omega)
+      simp [Circuit.eval_map, h]
+
+/--
+Build the circuit of evaluation at [0..n+1],
+usig the circuit of evaluation at [0..n] and the
+circuit of evaluation at 'n+1'.
+-/
+def mkEvalWithNCircuitSucc_of_mkEvalWithNCircuit_mkEvalWithCircuit_succ {arity : Type _}
+    [DecidableEq arity] [Fintype arity] [Hashable arity]
+    (p : FSM arity) (n : Nat)
+    (mkEvalWith : Circuit (Vars p.α arity (n + 2)))
+    (hMkEvalWith : Circuit.Equiv mkEvalWith (mkEvalWithCircuit p (n + 1)))
+    (mkEvalWithN : Circuit (Vars p.α arity (n + 1)))
+    (hMkEvalWithN : Circuit.Equiv mkEvalWithN (mkEvalWithNCircuit p n))
+     :
+    { c : Circuit (Vars p.α arity (n + 2)) //
+      Circuit.Equiv c (mkEvalWithNCircuit p (n + 1)) } where
+  val :=  mkEvalWithN.map (fun v => v.castLe (by omega)) ||| mkEvalWith
+  property := by
+    ext env
+    rw [mkEvalWithNCircuit_succ_Eqiv_mkEvalWithNCircuit_or]
+    simp [Circuit.eval_map]
+    rw [hMkEvalWithN, hMkEvalWith]
 
 @[simp]
 theorem eval_mkEvalWithNCircuit_eq_false_iff
@@ -1386,7 +1208,163 @@ theorem eval_mkEvalWithNCircuit_eq_true_iff
     apply Iff.not
     apply eval_mkEvalWithNCircuit_eq_false_iff (hEnvBitstream := hEnvBitstream)
 
+/--
+Make the circuit that sets the state vector to be the init carry of the FSM.
+-/
+def mkCircuitWithInitCarry {arity : Type _}
+    [DecidableEq arity]
+    [Fintype arity]
+    [Hashable arity]
+    (p : FSM arity) {n : Nat} (evalCirc : Circuit (Vars p.α arity n)) : Circuit (Vars Empty arity n) :=
+  evalCirc.bind fun v =>
+    match v with
+    | .state s => Circuit.ofBool (p.initCarry s)
+    | .inputs i => Circuit.var true (Vars.inputs i)
 
+/-- Show how 'mkCircuitWithInitCarry' evaluates the circuit with respect to an
+arbitrary environment: It substitutes the state vector with the initCarry,
+and leaves other data alone. -/
+@[simp]
+theorem mkCircuitWithInitCarry_eval_eq {arity : Type _}
+    [DecidableEq arity]
+    [Fintype arity]
+    [Hashable arity]
+    (p : FSM arity) {n : Nat}
+    (evalCirc : Circuit (Vars p.α arity n))
+    (envBool : Vars Empty arity n → Bool) :
+  (mkCircuitWithInitCarry p evalCirc).eval envBool =
+  evalCirc.eval (fun v =>
+    match v with
+    | .state s => p.initCarry s
+    | .inputs i => envBool (.inputs i)) := by
+  simp [mkCircuitWithInitCarry]
+  simp [Circuit.eval_bind, Circuit.eval_map]
+  congr
+  funext x
+  rcases x with a | i
+  · simp only [Circuit.eval, ↓reduceIte, Vars.state]
+    rcases p.initCarry a <;> simp
+  · simp only [Circuit.eval, ↓reduceIte, Vars.inputs]
+
+
+/--
+Make the circuit that evaluates the FSM at step 'n',
+in terms of 'mkEvalWithCircuit'.
+-/
+def mkEvalCircuit' {arity : Type _}
+    [DecidableEq arity]
+    [Fintype arity]
+    [Hashable arity]
+    (p : FSM arity) (n : Nat) :
+    Circuit (Vars Empty arity (n + 1)) :=
+  mkCircuitWithInitCarry p (mkEvalWithCircuit p n)
+
+/--
+we show that `mkEvalCircuit'` equals
+-/
+@[simp]
+theorem eval_mkEvalCircuit'_eq
+    {arity : Type _}
+    [DecidableEq arity]
+    [Fintype arity]
+    [Hashable arity]
+    (p : FSM arity) (n : Nat)
+    (envBool : Vars Empty arity (n + 1) → Bool)
+    (envBitstream : arity → BitStream)
+    (hEnvBitstream : EnvOutRelated envBool envBitstream) :
+    -- Make a safety circuit, that computes the evaluation of the FSM.
+    (mkEvalCircuit' p n).eval envBool =
+      p.eval envBitstream n  := by
+  simp [mkEvalCircuit']
+  rw [eval_mkEvalWithCircuit_eq (envBitstream := envBitstream)]
+  · rw [FSM.evalWith_eq_eval_of_eq_init]
+    funext x
+    simp
+  · constructor
+    intros x i hi
+    simp only [Fin.castSucc_mk]
+    apply hEnvBitstream.envBool_inputs_mk_eq_envBitStream
+
+/-- Make the list of safety circuits upto length 'n + 1'. -/
+def mkSafetyCircuitAuxList {arity : Type _}
+    [DecidableEq arity]
+    [Fintype arity]
+    [Hashable arity]
+    (p : FSM arity) (n : Nat) :
+    List (Circuit (Vars Empty arity (n+1))) :=
+  let ys := (List.range (n+1)).attach
+  ys.map fun i =>
+    (mkEvalCircuit' p i.val).map (fun vs => vs.castLe (by
+      have := i.property; simp at this; omega
+    ))
+
+/--
+the circuit that witnesses safety for (n+1),
+by building an arbitrary safety circuit, and
+then using the carry circuit to set the state vector.
+-/
+def mkSafetyCircuit' {arity : Type _}
+    [DecidableEq arity] [Fintype arity] [Hashable arity]
+    (p : FSM arity) (n : Nat) :
+    Circuit (Vars Empty arity (n + 1)) :=
+  mkCircuitWithInitCarry p (mkEvalWithNCircuit p n)
+
+/--
+This tells us that mkSafetyCircuit' evaluates to false
+iff the underlying FSM is unsafe up to n steps.
+-/
+theorem eval_mkSafetyCircuit'_eq_false_iff_ {arity : Type _}
+    [DecidableEq arity] [Fintype arity] [Hashable arity]
+    (p : FSM arity) (n : Nat)
+    (envBool : Vars Empty arity (n + 1) → Bool)
+    (envBitstream : arity → BitStream)
+    (hEnvBitstream : EnvOutRelated envBool envBitstream) :
+    (mkSafetyCircuit' p n).eval envBool = false ↔
+    (∀ i ≤ n, p.eval envBitstream i = false) := by
+  rw [mkSafetyCircuit']
+  rw [mkCircuitWithInitCarry_eval_eq]
+  rw [eval_mkEvalWithNCircuit_eq_false_iff]
+  constructor
+  · intros h i hi
+    apply h
+    omega
+  · intros hCirc i hi
+    apply hCirc
+    omega
+  · constructor
+    intros x j hj
+    apply hEnvBitstream.envBool_inputs_mk_eq_envBitStream
+
+@[simp]
+theorem mkSafetyCircuit'_eval_eq_false_iff {arity : Type _}
+    [DecidableEq arity] [Fintype arity] [Hashable arity]
+    (p : FSM arity) (n : Nat) :
+    (∀ envBool, (mkSafetyCircuit' p n).eval envBool = false) ↔
+    (∀ envBitstream, ∀ i ≤ n, p.eval envBitstream i = false) := by
+  constructor
+  · intros h envBitstream i hi
+    let envBool := envBoolEmpty_of_envBitstream envBitstream n
+    specialize h envBool
+    rw [eval_mkSafetyCircuit'_eq_false_iff_
+      (envBitstream := envBitstream)
+    ] at h
+    · apply h
+      omega
+    · simp [envBool]
+  · intros hCirc envBool
+    rw [eval_mkSafetyCircuit'_eq_false_iff_
+      (envBitstream := Bitstream_of_envBool envBool)
+    ]
+    · intros i hi
+      apply hCirc (Bitstream_of_envBool envBool) i hi
+    · simp
+
+/-! ## Arbitrary State Vector Builder
+
+This section builds a circuit that produces the state vector after 'n' iterations,
+starting with a state vector that is given by the circuit itself.
+
+-/
 
 def mkUnsatImpliesCircuit (lhs rhs : Circuit α) : Circuit α :=
   -- truth table of this circuit:
@@ -1420,6 +1398,7 @@ def mkIndHypCircuit {arity : Type _}
   mkUnsatImpliesCircuit
     ((mkEvalWithNCircuit p n).map (fun vs => vs.castLe (by omega)))
     (mkEvalWithNCircuit p (n + 1))
+
 
 /-- induction hyp circuit. -/
 theorem eval_mkIndHypCircuit_eq_false_iff_ {arity : Type _}
@@ -1495,19 +1474,6 @@ theorem eval_mkIndHypCircuit_eq_false_iff {arity : Type _}
       · omega
     · simp
 
-@[simp]
-theorem Inputs.castLe_eq_self {α : Type _} {n : Nat} (i : Inputs α n) (h : n ≤ n) :
-    i.castLe h = i := by
-  simp [Inputs.castLe]
-
-/-- casting to the same width equals vars-/
-@[simp]
-theorem Vars.castLe_eq_self {α : Type _} {n : Nat} (v : Vars α σ n) (h : n ≤ n) :
-    v.castLe h = v := by
-  rcases v with x | i
-  · simp [Vars.castLe]
-  · simp [Vars.castLe]
-
 /-- induction principle with a uniform bound 'bound' in place. -/
 @[elab_as_elim]
 theorem ind_principle₂  {motive : Nat → Prop} (bound : Nat)
@@ -1537,11 +1503,11 @@ theorem ind_principle₂  {motive : Nat → Prop} (bound : Nat)
     [Fintype arity]
     [Hashable arity]
     (p : FSM arity)
-    (hs : (mkSafetyCircuit p n).always_false)
+    (hs : (mkSafetyCircuit' p n).always_false)
     (hind : (mkIndHypCircuit p n).always_false) :
     ∀ (envBitstream : arity → BitStream) (i : Nat), p.eval envBitstream i = false := by
   intros envBitstream i
-  simp [eval_mkSafetyCircuit_eq_false_iff] at hs
+  simp only [Circuit.always_false_iff, Bool.not_eq_true, mkSafetyCircuit'_eval_eq_false_iff] at hs
   simp [eval_mkIndHypCircuit_eq_false_iff] at hind
   rw [FSM.eval_eq_evalWith_initCarry]
   induction i using Nat.strong_induction_on
@@ -1583,7 +1549,7 @@ theorem eval_eq_false_of_verifyAIG_eq_of_verifyAIG_eq
     [Hashable arity]
     {p : FSM arity}
     (sCert : BVDecide.Frontend.LratCert)
-    (hs : verifyCircuit (mkSafetyCircuit p n) sCert = true)
+    (hs : verifyCircuit (mkSafetyCircuit' p n) sCert = true)
     (indCert : BVDecide.Frontend.LratCert)
     (hind : verifyCircuit (mkIndHypCircuit p n) indCert = true) :
     ∀ env i, p.eval env i = false := by
@@ -1600,7 +1566,7 @@ theorem _root_.Predicate.denote_of_verifyAIG_of_verifyAIG
     (p : Predicate)
     (n : Nat)
     (sCert : BVDecide.Frontend.LratCert)
-    (hs : verifyCircuit (mkSafetyCircuit (predicateEvalEqFSM p).toFSM n) sCert = true)
+    (hs : verifyCircuit (mkSafetyCircuit' (predicateEvalEqFSM p).toFSM n) sCert = true)
     (indCert : BVDecide.Frontend.LratCert)
     (hind : verifyCircuit (mkIndHypCircuit (predicateEvalEqFSM p).toFSM n) indCert = true) :
     p.denote w vars := by
@@ -1630,65 +1596,289 @@ def isSuccess : DecideIfZerosOutput → Bool
 end DecideIfZerosOutput
 
 
+-- @[nospecialize]
+-- partial def decideIfZerosAuxVerified {arity : Type _}
+--     [DecidableEq arity] [Fintype arity] [Hashable arity]
+--     (iter : Nat) (maxIter : Nat)
+--     (fsm : FSM arity) :
+--     TermElabM (DecideIfZerosOutput) := do
+--   trace[Bits.FastVerif] s!"K-induction (iter={iter})"
+--   if iter ≥ maxIter && maxIter != 0 then
+--     throwError s!"ran out of iterations, quitting"
+--     return .exhaustedIterations maxIter
+--   let tStart ← IO.monoMsNow
+--   let cSafety : Circuit (Vars Empty arity (iter+1)) := mkSafetyCircuit' fsm iter
+--   let tEnd ← IO.monoMsNow
+--   let tElapsedSec := (tEnd - tStart) / 1000
+--   trace[Bits.FastVerif] m!"Built safety circuit in '{tElapsedSec}s'"
+
+--   let formatα : fsm.α → Format := fun s => "s" ++ formatDecEqFinset s
+--   let formatEmpty : Empty → Format := fun e => e.elim
+--   let formatArity : arity → Format := fun i => "i" ++ formatDecEqFinset i
+--   trace[Bits.FastVerif] m!"safety circuit: {formatCircuit (Vars.format formatEmpty formatArity) cSafety}"
+--   let tStart ← IO.monoMsNow
+--   let safetyCert? ← checkCircuitUnsatAux cSafety
+--   let tEnd ← IO.monoMsNow
+--   let tElapsedSec := (tEnd - tStart) / 1000
+--   trace[Bits.FastVerif] m!"Checked safety property in {tElapsedSec} seconds."
+--   match safetyCert? with
+--   | .none =>
+--     trace[Bits.FastVerif] s!"Safety property failed on initial state."
+--     return .safetyFailure iter
+--   | .some safetyCert =>
+--     trace[Bits.FastVerif] s!"Safety property succeeded on initial state. Building induction circuit..."
+
+--     let tStart ← IO.monoMsNow
+--     let cIndHyp := mkIndHypCircuit fsm iter
+--     let tEnd ← IO.monoMsNow
+--     let tElapsedSec := (tEnd - tStart) / 1000
+--     trace[Bits.FastVerif] m!"Built induction circuit in '{tElapsedSec}s'"
+
+--     let tStart ← IO.monoMsNow
+--     trace[Bits.FastVerif] m!"induction circuit: {formatCircuit (Vars.format formatα formatArity) cIndHyp}"
+--     -- let le : Bool := sorry
+--     let indCert? ← checkCircuitUnsatAux cIndHyp
+--     let tEnd ← IO.monoMsNow
+--     let tElapsedSec := (tEnd - tStart) / 1000
+--     trace[Bits.FastVerif] s!"Checked inductive invariant in '{tElapsedSec}s'."
+--     match indCert? with
+--     | .some indCert =>
+--       trace[Bits.FastVerif] s!"Inductive invariant established."
+--       return .proven iter safetyCert indCert
+--     | .none =>
+--       trace[Bits.FastVerif] s!"Unable to establish inductive invariant. Trying next iteration ({iter+1})..."
+--       decideIfZerosAuxVerified (iter + 1) maxIter fsm
+
+/-- structure for incrementally building the k-induction circuits. -/
+structure KInductionCircuits {arity : Type _}
+  [DecidableEq arity] [Fintype arity] [Hashable arity] (fsm : FSM arity) (n : Nat) where
+  cCarryWith : fsm.α → Circuit (Vars fsm.α arity n)
+  hCarryWith : ∀ (a : fsm.α),
+    Circuit.Equiv (cCarryWith a) (mkCarryWithCircuit fsm n a)
+  cEvalWithN : Circuit (Vars fsm.α arity (n + 1))
+  hEvalWithN : Circuit.Equiv cEvalWithN (mkEvalWithNCircuit fsm n)
+
+namespace KInductionCircuits
+/-- Make the carry circuit for the k-induction circuits. -/
+def mkZero {arity : Type _}
+    [DecidableEq arity] [Fintype arity] [Hashable arity]
+    (fsm : FSM arity) :
+    KInductionCircuits fsm 0 where
+  cCarryWith := mkCarryWithCircuit fsm 0
+  hCarryWith := by intros a; simp
+  cEvalWithN := mkEvalWithNCircuit fsm 0
+  hEvalWithN := by simp
+
+
+/-- make the 'carryWith' circuit of the successor, by using the current
+circuit state. -/
+def mkSuccCarryWith {arity : Type _}
+    [DecidableEq arity] [Fintype arity] [Hashable arity]
+    (fsm : FSM arity) (n : Nat)
+    (prev : KInductionCircuits fsm n) :
+    { f : fsm.α → Circuit (Vars fsm.α arity (n + 1)) //
+      ∀ (a : fsm.α), Circuit.Equiv (f a) (mkCarryWithCircuit fsm (n + 1) a) } :=
+  mkCarryWithSuccCircuit fsm n prev.cCarryWith prev.hCarryWith
+
+/--
+make the 'evalWith' circuit of the successor, by using the current
+circuit state.
+-/
+def mkSuccEvalWith {arity : Type _}
+    [DecidableEq arity] [Fintype arity] [Hashable arity]
+    (fsm : FSM arity) (n : Nat)
+    (prev : KInductionCircuits fsm n) :
+    { c : Circuit (Vars fsm.α arity (n + 2)) //
+      Circuit.Equiv c (mkEvalWithCircuit fsm (n + 1)) } :=
+  let carry := mkSuccCarryWith fsm n prev
+  mkEvalWithCircuit_of_mkCarryWithCircuit fsm (n + 1)
+    carry.val carry.prop
+
+/-- make the 'evalWithN' circuit for the (n+1)th iteration. -/
+def mkSuccEvalWithN {arity : Type _}
+    [DecidableEq arity] [Fintype arity] [Hashable arity]
+    (fsm : FSM arity) (n : Nat)
+    (prev : KInductionCircuits fsm n) :
+    { c : Circuit (Vars fsm.α arity (n + 2)) //
+      Circuit.Equiv c (mkEvalWithNCircuit fsm (n + 1)) } :=
+  let c := mkSuccEvalWith fsm n prev
+  mkEvalWithNCircuitSucc_of_mkEvalWithNCircuit_mkEvalWithCircuit_succ
+    fsm n c.val c.prop prev.cEvalWithN prev.hEvalWithN
+
+-- NOTE [Circuit Equivalence As a quotient]:
+-- We ideally should have a notion of `Circuit.equiv`, which says that
+-- circuits are equivalent if they denote the same function.
+--
+-- However, for now, don't bother. We change the direction we compute the `bigOr`
+-- of the circuits, so that the latest circuit is the one that is at the outermost
+-- layer of the `bigOr`. This way, we can stick a new circuit as
+-- `circUptoN+1 = circN+1 || (...circUptoN...)`.
+
+def mkSucc {arity : Type _}
+    [DecidableEq arity] [Fintype arity] [Hashable arity]
+    (fsm : FSM arity)
+    (prev : KInductionCircuits fsm n) :
+    KInductionCircuits fsm (n + 1) :=
+  let cCarryWith := mkCarryWithSuccCircuit fsm n
+      prev.cCarryWith prev.hCarryWith
+  let hCarryWith := cCarryWith.property
+  let cEvalWithN := mkSuccEvalWithN fsm n prev
+  let hEvalWithN := cEvalWithN.property
+  { cCarryWith,
+    hCarryWith,
+    cEvalWithN,
+    hEvalWithN
+  }
+
+
+/- Make the n'th k-induction circuit family. -/
+def mkN {arity : Type _}
+    [DecidableEq arity] [Fintype arity] [Hashable arity]
+    (fsm : FSM arity) (n : Nat) :
+    KInductionCircuits fsm n :=
+    match n with
+    | 0 => mkZero fsm
+    | n + 1 => (mkN fsm n).mkSucc
+
+/-- Make the safety circuit, incrementally. -/
+def mkSafetyCircuit {arity : Type _}
+    [DecidableEq arity] [Fintype arity] [Hashable arity]
+    {fsm : FSM arity} (circs : KInductionCircuits fsm n) :
+    { c : Circuit (Vars Empty arity (n + 1)) //
+    Circuit.Equiv c (mkSafetyCircuit' fsm n) } :=
+  let circ := mkCircuitWithInitCarry fsm circs.cEvalWithN
+  ⟨circ, by
+    rw [mkSafetyCircuit']
+    subst circ
+    ext env
+    simp only [mkCircuitWithInitCarry_eval_eq]
+    rw [circs.hEvalWithN]
+  ⟩
+
+/-- Make the induction hypothesis circuit, incrementally. -/
+def mkIndHypCircuit {arity : Type _}
+    [DecidableEq arity] [Fintype arity] [Hashable arity]
+    {fsm : FSM arity} (circs : KInductionCircuits fsm n) :
+    { c : Circuit (Vars fsm.α arity (n + 2)) //
+    Circuit.Equiv c (mkIndHypCircuit fsm n) } :=
+  let circ := mkUnsatImpliesCircuit
+    (circs.cEvalWithN.map (fun vs => vs.castLe (by omega)))
+    circs.mkSuccEvalWithN.val
+  ⟨circ, by
+    rw [BvDecide.mkIndHypCircuit]
+    subst circ
+    ext env
+    simp [mkUnsatImpliesCircuit, Circuit.eval_map]
+    rw [circs.hEvalWithN]
+    rw [circs.mkSuccEvalWithN.prop]
+  ⟩
+
+  theorem eval_eq_false_of_mkN_mkIndHypCircuit_false_of_mkN_mkSafetyCircuit_false {n : Nat}
+    {arity : Type _}
+    [DecidableEq arity]
+    [Fintype arity]
+    [Hashable arity]
+    (p : FSM arity)
+    (hs : (KInductionCircuits.mkN p n).mkSafetyCircuit.val.always_false)
+    (hind : (KInductionCircuits.mkN p n).mkIndHypCircuit.val.always_false) :
+    ∀ (envBitstream : arity → BitStream) (i : Nat), p.eval envBitstream i = false := by
+  apply BvDecide.eval_eq_false_of_mkIndHypCircuit_false_of_mkSafetyCircuit_false (n := n)
+  · rw [Circuit.always_false_iff] at hs hind ⊢
+    intros env
+    rw [← (mkN p n).mkSafetyCircuit.prop]
+    simp [hs env]
+  · rw [Circuit.always_false_iff] at hs hind ⊢
+    intros env
+    rw [← (mkN p n).mkIndHypCircuit.prop]
+    simp [hind env]
+
+/-- Prove that predicate is true iff the cerritificates check out. -/
+theorem _root_.Predicate.denote_of_verifyAIG_of_verifyAIG'
+    {w : Nat}
+    {vars : List (BitVec w)}
+    (p : Predicate)
+    (n : Nat)
+    (sCert : BVDecide.Frontend.LratCert)
+    (hs : verifyCircuit (mkN (predicateEvalEqFSM p).toFSM n).mkSafetyCircuit.val sCert = true)
+    (indCert : BVDecide.Frontend.LratCert)
+    (hind : verifyCircuit (mkN (predicateEvalEqFSM p).toFSM n).mkIndHypCircuit.val indCert = true) :
+    p.denote w vars := by
+  apply Predicate.denote_of_eval
+  rw [← Predicate.evalFin_eq_eval p
+    (varsList := (List.map BitStream.ofBitVec vars))
+    (varsFin := fun i => (List.map BitStream.ofBitVec vars).getD i default)]
+  · rw [(predicateEvalEqFSM p).good]
+    apply eval_eq_false_of_mkN_mkIndHypCircuit_false_of_mkN_mkSafetyCircuit_false (n := n)
+    · rw [always_false_of_verifyCircuit]
+      rw [hs]
+    · rw [always_false_of_verifyCircuit]
+      rw [hind]
+  · intros i
+    simp
+
+end KInductionCircuits
+
 @[nospecialize]
-partial def decideIfZerosAuxVerified {arity : Type _}
+partial def decideIfZerosAuxVerified' {arity : Type _}
     [DecidableEq arity] [Fintype arity] [Hashable arity]
     (iter : Nat) (maxIter : Nat)
-    (fsm : FSM arity) :
+    (fsm : FSM arity)
+    (circs : KInductionCircuits fsm iter) :
     TermElabM (DecideIfZerosOutput) := do
-  trace[Bits.FastVerif] s!"K-induction (iter={iter})"
-  if iter ≥ maxIter && maxIter != 0 then
-    throwError s!"ran out of iterations, quitting"
-    return .exhaustedIterations maxIter
-  let tStart ← IO.monoMsNow
-  let cSafety : Circuit (Vars Empty arity (iter+1)) := mkSafetyCircuit fsm iter
-  let tEnd ← IO.monoMsNow
-  let tElapsedSec := (tEnd - tStart) / 1000
-  trace[Bits.FastVerif] m!"Built safety circuit in '{tElapsedSec}s'"
-
-  let formatα : fsm.α → Format := fun s => "s" ++ formatDecEqFinset s
-  let formatEmpty : Empty → Format := fun e => e.elim
-  let formatArity : arity → Format := fun i => "i" ++ formatDecEqFinset i
-  trace[Bits.FastVerif] m!"safety circuit: {formatCircuit (Vars.format formatEmpty formatArity) cSafety}"
-  let tStart ← IO.monoMsNow
-  let safetyCert? ← checkCircuitUnsatAux cSafety
-  let tEnd ← IO.monoMsNow
-  let tElapsedSec := (tEnd - tStart) / 1000
-  trace[Bits.FastVerif] m!"Checked safety property in {tElapsedSec} seconds."
-  match safetyCert? with
-  | .none =>
-    trace[Bits.FastVerif] s!"Safety property failed on initial state."
-    return .safetyFailure iter
-  | .some safetyCert =>
-    trace[Bits.FastVerif] s!"Safety property succeeded on initial state. Building induction circuit..."
-
+  withTraceNode `trace.Bits.Fast (fun _ => return s!"K-induction (iter={iter})") do
+    if iter ≥ maxIter && maxIter != 0 then
+      throwError s!"ran out of iterations, quitting"
+      return .exhaustedIterations maxIter
     let tStart ← IO.monoMsNow
-    let cIndHyp := mkIndHypCircuit fsm iter
+    let cSafety : Circuit (Vars Empty arity (iter+1)) := circs.mkSafetyCircuit.val
     let tEnd ← IO.monoMsNow
     let tElapsedSec := (tEnd - tStart) / 1000
-    trace[Bits.FastVerif] m!"Built induction circuit in '{tElapsedSec}s'"
+    trace[Bits.FastVerif] m!"Built new safety circuit in '{tElapsedSec}s'"
 
+    let formatα : fsm.α → Format := fun s => "s" ++ formatDecEqFinset s
+    let formatEmpty : Empty → Format := fun e => e.elim
+    let formatArity : arity → Format := fun i => "i" ++ formatDecEqFinset i
+    trace[Bits.FastVerif] m!"safety circuit: {formatCircuit (Vars.format formatEmpty formatArity) cSafety}"
     let tStart ← IO.monoMsNow
-    trace[Bits.FastVerif] m!"induction circuit: {formatCircuit (Vars.format formatα formatArity) cIndHyp}"
-    -- let le : Bool := sorry
-    let indCert? ← checkCircuitUnsatAux cIndHyp
+    let safetyCert? ← checkCircuitUnsatAux cSafety
     let tEnd ← IO.monoMsNow
     let tElapsedSec := (tEnd - tStart) / 1000
-    trace[Bits.FastVerif] s!"Checked inductive invariant in '{tElapsedSec}s'."
-    match indCert? with
-    | .some indCert =>
-      trace[Bits.FastVerif] s!"Inductive invariant established."
-      return .proven iter safetyCert indCert
+    trace[Bits.FastVerif] m!"Checked safety property in {tElapsedSec} seconds."
+    match safetyCert? with
     | .none =>
-      trace[Bits.FastVerif] s!"Unable to establish inductive invariant. Trying next iteration ({iter+1})..."
-      decideIfZerosAuxVerified (iter + 1) maxIter fsm
+      trace[Bits.FastVerif] s!"Safety property failed on initial state."
+      return .safetyFailure iter
+    | .some safetyCert =>
+      trace[Bits.FastVerif] s!"Safety property succeeded on initial state. Building induction circuit..."
+
+      let tStart ← IO.monoMsNow
+      let cIndHyp := circs.mkIndHypCircuit
+      let tEnd ← IO.monoMsNow
+      let tElapsedSec := (tEnd - tStart) / 1000
+      trace[Bits.FastVerif] m!"Built induction circuit in '{tElapsedSec}s'"
+
+      let tStart ← IO.monoMsNow
+      trace[Bits.FastVerif] m!"induction circuit: {formatCircuit (Vars.format formatα formatArity) cIndHyp.val}"
+      -- let le : Bool := sorry
+      let indCert? ← checkCircuitUnsatAux cIndHyp.val
+      let tEnd ← IO.monoMsNow
+      let tElapsedSec := (tEnd - tStart) / 1000
+      trace[Bits.FastVerif] s!"Checked inductive invariant in '{tElapsedSec}s'."
+      match indCert? with
+      | .some indCert =>
+        trace[Bits.FastVerif] s!"Inductive invariant established."
+        return .proven iter safetyCert indCert
+      | .none =>
+        trace[Bits.FastVerif] s!"Unable to establish inductive invariant. Trying next iteration ({iter+1})..."
+    decideIfZerosAuxVerified' (iter + 1) maxIter fsm  circs.mkSucc
+
 
 @[nospecialize]
-def _root_.FSM.decideIfZerosVerified  {arity : Type _} [DecidableEq arity]  [Fintype arity] [Hashable arity]
+def _root_.FSM.decideIfZerosVerified {arity : Type _} [DecidableEq arity]  [Fintype arity] [Hashable arity]
    (fsm : FSM arity) (maxIter : Nat) : TermElabM DecideIfZerosOutput :=
   -- decideIfZerosM Circuit.impliesCadical fsm
   withTraceNode `trace.Bits.Fast (fun _ => return "k-induction") (collapsed := false) do
-    decideIfZerosAuxVerified 0 maxIter fsm
+    decideIfZerosAuxVerified' 0 maxIter fsm (KInductionCircuits.mkZero fsm)
 
 end BvDecide
 
